ThymeTests/Imported.lean
@@ -7,11 +7,11 @@ open Thyme
 public section
 
 @[expose]
-def importedSucc (x : Code Nat) : Code Nat :=
+def importedSucc [Staged] (x : Code Nat) : Code Nat :=
   `⟨~x + 1⟩
 
 /-- A non-exposed definition used to test coherence diagnostics across module boundaries. -/
-def opaqueImportedSucc (x : Code Nat) : Code Nat :=
+def opaqueImportedSucc [Staged] (x : Code Nat) : Code Nat :=
   `⟨~x + 1⟩
 
 end
